CollapsingTowers/TwoLevelRec/SyntacticTyping/Env.lean
@@ -1,0 +1,32 @@
+import CollapsingTowers.TwoLevelRec.SyntacticTyping.Ty
+import CollapsingTowers.TwoLevelRec.Utils.Defs
+
+abbrev TEnv :=
+  List (Ty × Stage)
+
+notation:max "⦰" => ([] : TEnv)
+
+@[simp]
+def erase_env : TEnv → TEnv
+  | [] => []
+  | (τ, _) :: Γ => (erase_ty τ, 𝟙) :: erase_env Γ
+
+lemma erase_env.length : ∀ Γ, Γ.length = (erase_env Γ).length :=
+  by
+  intros Γ
+  induction Γ
+  case nil => rfl
+  case cons IH => simp; apply IH
+
+lemma erase_env.binds : ∀ x τ 𝕊 Γ, binds x (τ, 𝕊) Γ → binds x (erase_ty τ, 𝟙) (erase_env Γ) :=
+  by
+  intros x τ 𝕊 Γ Hbinds
+  induction Γ
+  case nil => nomatch Hbinds
+  case cons tails IH =>
+    by_cases HEq : tails.length = x
+    . simp [if_pos HEq] at Hbinds
+      simp [← erase_env.length, if_pos HEq, Hbinds]
+    . simp [if_neg HEq] at Hbinds
+      simp [← erase_env.length, if_neg HEq]
+      apply IH; apply Hbinds
