CollapsingTowers/TwoLevelRec/SyntacticTyping/EraseSafety.lean
@@ -1,0 +1,102 @@
+import CollapsingTowers.TwoLevelRec.SyntacticTyping.Typing
+
+-- Γ ⊢ e : τ
+-- ————————————————
+-- ‖Γ‖ ⊢ ‖e‖ : ‖τ‖
+theorem typing.erase_safety : ∀ Γ 𝕊 e τ φ, typing Γ 𝕊 e τ φ → typing (erase_env Γ) 𝟙 ‖e‖ (erase_ty τ) ⊥ :=
+  by
+  intros Γ 𝕊 e τ φ Hτ
+  apply
+    @typing.rec
+      (fun Γ 𝕊 e τ φ (H : typing Γ 𝕊 e τ φ) => typing (erase_env Γ) 𝟙 ‖e‖ (erase_ty τ) ⊥)
+      (fun Γ e τ φ (H : typing_reification Γ e τ φ) => typing (erase_env Γ) 𝟙 ‖e‖ (erase_ty τ) ⊥)
+  <;> intros
+  case fvar Hbinds _ =>
+    apply typing.fvar
+    . apply erase_env.binds; apply Hbinds
+    . apply grounded_ty.under_erase
+  case lam Hwbt Hclosed IH =>
+    apply typing.lam
+    . rw [← erase_env.length, ← comm.erase_opening]
+      apply IH
+    . apply grounded_ty.under_erase
+    . rw [← erase_env.length, ← closed.under_erase]
+      apply Hclosed
+  case lift_lam IH => apply IH
+  case app₁ IHf IHarg =>
+    rw [← Effect.union_pure ⊥, ← Effect.union_pure (⊥ ∪ ⊥)]
+    apply typing.app₁
+    . apply IHf
+    . apply IHarg
+  case app₂ IHf IHarg =>
+    rw [← Effect.union_pure ⊥, ← Effect.union_pure (⊥ ∪ ⊥)]
+    apply typing.app₁
+    . apply IHf
+    . apply IHarg
+  case lit => apply typing.lit
+  case lift_lit IH => apply IH
+  case binary₁ IHl IHr =>
+    rw [← Effect.union_pure ⊥]
+    apply typing.binary₁
+    . apply IHl
+    . apply IHr
+  case binary₂ IHl IHr =>
+    rw [← Effect.union_pure ⊥]
+    apply typing.binary₁
+    . apply IHl
+    . apply IHr
+  case code_fragment x _ Hbinds Hwbt =>
+    apply typing.fvar
+    . simp; apply erase_env.binds; apply Hbinds
+    . apply grounded_ty.under_erase
+  case code_rep IH => apply IH
+  case reflect IH => apply IH
+  case lam𝕔 Hclosed IH =>
+    apply typing.lam
+    . rw [← erase_env.length, ← comm.erase_opening]
+      apply IH
+    . apply grounded_ty.under_erase
+    . rw [← erase_env.length, ← closed.under_erase]
+      apply Hclosed
+  case lets Hclosed IHb IHe =>
+    rw [← Effect.union_pure ⊥]
+    apply typing.lets
+    . apply IHb
+    . rw [← erase_env.length, ← comm.erase_opening]
+      apply IHe
+    . apply grounded_ty.under_erase
+    . rw [← erase_env.length, ← closed.under_erase]
+      apply Hclosed
+  case lets𝕔 Hclosed IHb IHe =>
+    rw [← Effect.union_pure ⊥]
+    apply typing.lets
+    . apply IHb
+    . rw [← erase_env.length, ← comm.erase_opening]
+      apply IHe
+    . apply grounded_ty.under_erase
+    . rw [← erase_env.length, ← closed.under_erase]
+      apply Hclosed
+  case run IH => apply IH
+  case fix₁ IH =>
+    apply typing.fix₁
+    . simp; rfl
+    . apply IH
+  case fix₂ IH =>
+    apply typing.fix₁
+    . simp; rfl
+    . apply IH
+  case ifz₁ IHc IHl IHr =>
+    rw [← Effect.union_pure ⊥, ← Effect.union_pure (⊥ ∪ ⊥)]
+    apply typing.ifz₁
+    . apply IHc
+    . apply IHl
+    . apply IHr
+  case ifz₂ IHc IHl IHr =>
+    rw [← Effect.union_pure ⊥, ← Effect.union_pure (⊥ ∪ ⊥)]
+    apply typing.ifz₁
+    . apply IHc
+    . apply IHl
+    . apply IHr
+  case pure IH => apply IH
+  case reify IH => apply IH
+  apply Hτ
